Checking in work done on lap-top while away to HCSS conference.

holsrcs/instantiationScript.sml
@@ -19,13 +19,15 @@ open statesTheory aggregatesTheory
 val _ = new_theory "instantiation"
 
 
-val _ = Hol_datatype`inst_record = <| typemap : string -> CPP_Type ;
-                                      tempmap : string -> CPP_ID ;
-                                      valmap : string -> TemplateValueArg |>`
+val _ = Hol_datatype`
+  inst_record = <| typemap : string -> CPP_Type ;
+                   tempmap : string -> bool # StaticField list # string ;
+                   valmap  : string -> TemplateValueArg 
+|>`
 
 val empty_inst_def = Define`
-  empty_inst = <| typemap := TypeID o IDVar;
-                  tempmap := IDVar;
+  empty_inst = <| typemap := (\s. TypeID (IDConstant(F,[],SFName s)));
+                  tempmap := (\s. (F, [], s)); 
                   valmap := TVAVar |>
 `;
 
@@ -45,80 +47,197 @@ val typeid_def = Define`
 `;
 val _ = export_rewrites ["typeid_def"]
 
+val IDhd_def = Define`
+  (IDhd (IDConstant(b, [], sf)) = sf) /\
+  (IDhd (IDConstant(b, h::t, sf)) = h)
+`;
+val _ = export_rewrites ["IDhd_def"]
 
-(* instantiate a type with template arguments *)
+val ID_updhd_def = Define`
+  (ID_updhd ty (IDConstant(b2, [], sf2)) = SOME ty) /\
+  (ID_updhd ty (IDConstant(b2, h::t, sf2)) = 
+     case typeid ty of 
+        NONE -> NONE
+     || SOME (IDConstant(b1,sfs1,sf1)) -> 
+          SOME (TypeID (IDConstant(b1, sfs1 ++ [sf1] ++ t, sf2))) 
+     || SOME (IDVar _) -> NONE)
+`;
+val _ = export_rewrites ["ID_updhd_def"]
+
+val dest_sfname_def = Define`
+  (dest_sfname (SFName s) = s) 
+`;
+val _ = export_rewrites ["dest_sfname_def"]
+
+val ID_updtemphd_def = Define`
+  (ID_updtemphd (b1,sfs1,sfn) targs (IDConstant(b2,[],sf2)) = 
+     SOME (TypeID (IDConstant(b1, sfs1, SFTempCall sfn targs)))) /\
+  (ID_updtemphd (b1,sfs1,sfn) targs (IDConstant(b2,h::t,sf2)) = 
+     SOME (TypeID 
+           (IDConstant(b1, 
+                       sfs1 ++ [SFTempCall sfn targs] ++ t, sf2)))) /\
+  (ID_updtemphd _ _ _ = NONE)
+`;
+val _ = export_rewrites ["ID_updtemphd_def"]
+
+val IDtl_def = Define`
+  IDtl (IDConstant(b, sfs, sf)) = sf
+`;
+
+val option_case_EQ_SOME = store_thm(
+  "option_case_EQ_SOME",
+  ``(option_case NONE f v = SOME v0) =
+        ?v0'. (v = SOME v0') /\ (f v0' = SOME v0)``,
+  Cases_on `v` THEN SRW_TAC [][]);
+val _ = export_rewrites ["option_case_EQ_SOME"]
+
+val olmap_ALL_MEM = store_thm(
+  "olmap_ALL_MEM",
+  ``!list x f. 
+        (olmap f list = SOME x) = 
+          (LENGTH x = LENGTH list) /\
+          !i. i < LENGTH list ==>
+              (f (EL i list) = SOME (EL i x))``,
+  Induct_on `list` THEN SRW_TAC [][] THENL [
+    SRW_TAC [][listTheory.LENGTH_NIL] THEN METIS_TAC [],
+    Cases_on `x` THEN SRW_TAC [][] THEN 
+    SRW_TAC [][EQ_IMP_THM] THENL [
+      Cases_on `i` THEN SRW_TAC [][] THEN FULL_SIMP_TAC (srw_ss()) [],
+      FIRST_X_ASSUM (Q.SPEC_THEN `0` MP_TAC) THEN SRW_TAC [][],
+      FIRST_X_ASSUM (Q.SPEC_THEN `SUC i` MP_TAC) THEN SRW_TAC [][]
+    ]
+  ]);
+
+val IDhd_inst_def = Define`
+  IDhd_inst sigma (b, sfs, sf) = 
+     if b then SOME (TypeID (IDConstant(b, sfs, sf)))
+     else 
+       case IDhd (IDConstant(F, sfs, sf)) of 
+          SFName s -> ID_updhd (sigma.typemap s) (IDConstant(F,sfs,sf))
+       || SFTempCall s targs -> 
+                      ID_updtemphd (sigma.tempmap s) targs 
+                                   (IDConstant(F,sfs,sf))
+`;
+
+val IDcases = store_thm(
+  "IDcases",
+  ``!i. (?b sfs sf. i = IDConstant(b,sfs,sf)) \/ (?nm. i = IDVar nm)``,
+  Cases THEN SRW_TAC [][] THEN 
+  Cases_on `p` THEN Cases_on `r` THEN SRW_TAC [][]);
+fun IDC_TAC q = Q.SPEC_THEN q FULL_STRUCT_CASES_TAC IDcases
+fun FSRW_TAC l = FULL_SIMP_TAC (srw_ss()) l
+
+val IDhd_inst_EQ_SOME = store_thm(
+  "IDhd_inst_EQ_SOME",
+  ``(IDhd_inst s (b,sfs,sf) = SOME ty) = 
+       b /\ (ty = TypeID (IDConstant(T,sfs,sf))) \/
+       ~b /\ (sfs = []) /\ 
+         (?s'. (sf = SFName s') /\ (ty = s.typemap s')) \/
+       ~b /\ (sfs = []) /\
+         (?s' tas b2 sfs2 sfn2. 
+             (sf = SFTempCall s' tas) /\ 
+             (s.tempmap s' = (b2, sfs2, sfn2)) /\
+             (ty = TypeID (IDConstant(b2,sfs2, SFTempCall sfn2 tas)))) \/
+       ~b /\ 
+         (?s' sfs1 sfs2 sf1 b'. 
+             (sfs = SFName s' :: sfs2) /\
+             (s.typemap s' = TypeID (IDConstant(b',sfs1,sf1))) /\
+             (ty = TypeID (IDConstant(b',sfs1 ++ [sf1] ++ sfs2,sf)))) \/
+       ~b /\ 
+         (?s' tas b2 sfs1 sfs2 sfn2.
+             (sfs = SFTempCall s' tas :: sfs2) /\
+             (s.tempmap s' = (b2,sfs1,sfn2)) /\
+             (ty = TypeID (IDConstant(b2,
+                                      sfs1 ++ [SFTempCall sfn2 tas] ++ sfs2,
+                                      sf))))``,
+  SRW_TAC [][IDhd_inst_def] THEN1 METIS_TAC [] THEN 
+  Cases_on `sfs` THENL [
+    SRW_TAC [][] THEN Cases_on `sf` THEN SRW_TAC [][] THENL [
+      Cases_on `s.tempmap s'` THEN Cases_on `r` THEN 
+      SRW_TAC [][] THEN METIS_TAC [],
+      METIS_TAC []
+    ],
+    SRW_TAC [][] THEN Cases_on `h` THEN SRW_TAC [][] THENL [
+      Cases_on `s.tempmap s'` THEN Cases_on `r` THEN SRW_TAC [][] THEN 
+      METIS_TAC [],
+      Cases_on `s.typemap s'` THEN SRW_TAC [][] THEN 
+      IDC_TAC `C''` THEN SRW_TAC [][] THEN METIS_TAC []
+    ]
+  ]);
+      
+(* the schema variable sigma is left out in order to get a nicer 
+   termination proof and induction principle *)
 val type_inst_defn = Hol_defn "type_inst" `
-  (type_inst sigma (TypeID cid) = cppid_inst sigma cid) /\
-  (type_inst sigma (Ptr ty) = OPTION_MAP Ptr (type_inst sigma ty)) /\
-  (type_inst sigma (MPtr nm ty) =
+  (type_inst (TypeID cid) = cppid_inst cid) /\
+  (type_inst (Ptr ty) = OPTION_MAP Ptr (type_inst ty)) /\
+  (type_inst (MPtr nm ty) =
      OP2CMB MPtr
-            (case cppid_inst sigma nm of NONE -> NONE || SOME ty -> typeid ty)
-            (type_inst sigma ty)) /\
-  (type_inst sigma (Ref ty) = OPTION_MAP Ref (type_inst sigma ty)) /\
-  (type_inst sigma (Array ty n) =
-     OPTION_MAP (\ty. Array ty n) (type_inst sigma ty)) /\
-  (type_inst sigma (Function ty tylist) =
-     OP2CMB Function (type_inst sigma ty) (olmap (type_inst sigma) tylist)) /\
-  (type_inst sigma (Const ty) = OPTION_MAP Const (type_inst sigma ty)) /\
-  (type_inst sigma (Class cid) = SOME (Class cid)) /\
-  (type_inst sigma ty = SOME ty)
+            (case cppid_inst nm of NONE -> NONE || SOME ty -> typeid ty)
+            (type_inst ty)) /\
+  (type_inst (Ref ty) = OPTION_MAP Ref (type_inst ty)) /\
+  (type_inst (Array ty n) =
+     OPTION_MAP (\ty. Array ty n) (type_inst ty)) /\
+  (type_inst (Function ty tylist) =
+     OP2CMB Function (type_inst ty) (olmap (type_inst) tylist)) /\
+  (type_inst (Const ty) = OPTION_MAP Const (type_inst ty)) /\
+  (type_inst (Class cid) = SOME (Class cid)) /\
+  (type_inst ty = SOME ty)
 
     /\
 
   (* id instantiation returns a type.  The type may just be a TypeID,
      possibly representing no change, or a "real" type. *)
-  (cppid_inst sigma (IDVar s) = SOME (sigma.typemap s)) /\
-  (cppid_inst sigma (IDConstant(b,sfs,sf)) =
-     case olmap (sfld_inst sigma) sfs of
-        NONE -> NONE
-     || SOME sfs' -> (case sfld_inst sigma sf of
-                         NONE -> NONE
-                      || SOME sf' -> SOME (TypeID (IDConstant(b,sfs',sf')))))
+  (cppid_inst (IDVar s) = SOME (TypeID (IDVar s))) /\
+  (cppid_inst (IDConstant(T,sfs,sf)) = 
+      case (olmap sfld_inst sfs, sfld_inst sf) of 
+         (NONE, NONE) -> NONE 
+      || (NONE, SOME sf') -> NONE
+      || (SOME sfs', NONE) -> NONE
+      || (SOME sfs', SOME sf') -> SOME (TypeID (IDConstant(T,sfs',sf')))) /\
+  (cppid_inst (IDConstant(F, sfs, sf)) = 
+      case (olmap sfld_inst sfs, sfld_inst sf) of 
+         (NONE, NONE) -> NONE
+      || (NONE, SOME sf') -> NONE
+      || (SOME sfs', NONE) -> NONE
+      || (SOME sfs', SOME sf') -> IDhd_inst sigma (F,sfs',sf'))
 
     /\
 
-  (temparg_inst sigma (TType ty) = OPTION_MAP TType (type_inst sigma ty)) /\
-  (temparg_inst sigma (TTemp tid) =
-     case cppid_inst sigma tid of
+  (temparg_inst (TType ty) = OPTION_MAP TType (type_inst ty)) /\
+  (temparg_inst (TTemp tid) =
+     case cppid_inst tid of
         NONE -> NONE
      || SOME ty -> OPTION_MAP TTemp (typeid ty)) /\
-  (temparg_inst sigma (TVal tva) =
-      OPTION_MAP TVal (temp_valarg_inst sigma tva))
+  (temparg_inst (TVal tva) =
+      OPTION_MAP TVal (temp_valarg_inst tva))
 
     /\
 
-  (temp_valarg_inst sigma (TNum i) = SOME (TNum i)) /\
-  (temp_valarg_inst sigma (TObj id) =
-      OPTION_MAP TObj (case cppid_inst sigma id of
+  (temp_valarg_inst (TNum i) = SOME (TNum i)) /\
+  (temp_valarg_inst (TObj id) =
+      OPTION_MAP TObj (case cppid_inst id of
                           NONE -> NONE
                        || SOME ty -> typeid ty)) /\
-  (temp_valarg_inst sigma (TMPtr id ty) =
+  (temp_valarg_inst (TMPtr id ty) =
       OP2CMB TMPtr
-             (case cppid_inst sigma id of NONE-> NONE || SOME ty -> typeid ty)
-             (type_inst sigma ty)) /\
-  (temp_valarg_inst sigma (TVAVar s) = SOME (sigma.valmap s))
+             (case cppid_inst id of NONE-> NONE || SOME ty -> typeid ty)
+             (type_inst ty)) /\
+  (temp_valarg_inst (TVAVar s) = SOME (sigma.valmap s))
 
     /\
 
-  (sfld_inst sigma (SFTempCall s targs) =
-      OPTION_MAP (SFTempCall s) (olmap (temparg_inst sigma) targs)) /\
-  (sfld_inst sigma (SFName s) = SOME (SFName s))
+  (sfld_inst (SFTempCall s targs) =
+      OPTION_MAP (SFTempCall s) (olmap (temparg_inst) targs)) /\
+  (sfld_inst (SFName s) = SOME (SFName s))
 `
 
 val (type_inst_def, type_inst_ind) = Defn.tprove(type_inst_defn,
-  WF_REL_TAC
-  `measure
-     (\a. case a of
-             INL (_, ty) -> CPP_Type_size ty
-          || INR (INL (_, id)) -> CPP_ID_size id
-          || INR (INR (INL (_, targ))) -> TemplateArg_size targ
-          || INR (INR (INR (INL (_, tva)))) ->
-               TemplateValueArg_size tva
-          || INR (INR (INR (INR (_, sfld)))) -> StaticField_size sfld)`
-     THEN
+  WF_REL_TAC `^(last (TotalDefn.guessR type_inst_defn))` THEN 
   SRW_TAC [ARITH_ss][] THENL [
     Induct_on `tylist` THEN SRW_TAC [][] THEN
     SRW_TAC [ARITH_ss][] THEN FULL_SIMP_TAC (srw_ss() ++ ARITH_ss) [],
+    Induct_on `sfs` THEN SRW_TAC [][] THEN
+    SRW_TAC [ARITH_ss][] THEN RES_TAC THEN DECIDE_TAC,
     Induct_on `sfs` THEN SRW_TAC [][] THEN
     SRW_TAC [ARITH_ss][] THEN RES_TAC THEN DECIDE_TAC,
     Induct_on `targs` THEN SRW_TAC [][] THEN
@@ -132,13 +251,29 @@ val _ = export_rewrites ["type_inst_def"]
 val type_match_def = Define`
   type_match ty1 ty2 = ?s. type_inst s ty1 = SOME ty2
 `;
-
 val _ = overload_on ("<=", ``type_match``);
 
 val olmap_EQ_NONE = prove(
   ``(olmap f list = NONE) = ?e. MEM e list /\ (f e = NONE)``,
   Induct_on `list` THEN SRW_TAC [][] THEN Cases_on `f h` THEN
   SRW_TAC [][] THEN METIS_TAC [TypeBase.distinct_of ``:'a option``]);
+
+val olmap_EQ_SOME = prove(
+  ``((olmap f list = SOME []) = (list = [])) /\
+    ((SOME [] = olmap f list) = (list = [])) /\
+    ((olmap f list = SOME (h::t)) = 
+        ?h0 t0. (f h0 = SOME h) /\ (list = h0::t0) /\ (olmap f t0 = SOME t))``,
+  Cases_on `list` THEN SRW_TAC [][]);
+
+val IDhd_inst_empty = store_thm(
+  "IDhd_inst_empty",
+  ``IDhd_inst empty_inst (b, sfs, sfld) = 
+      SOME (TypeID (IDConstant(b, sfs, sfld)))``,
+  SRW_TAC [][IDhd_inst_def] THEN Cases_on `sfs` THEN SRW_TAC [][] THENL [
+    Cases_on `sfld` THEN SRW_TAC [][empty_inst_def],
+    Cases_on `h` THEN SRW_TAC [][empty_inst_def]
+  ]);
+val _ = export_rewrites ["IDhd_inst_empty"]
 
 val type_inst_empty = store_thm(
   "type_inst_empty",
@@ -147,24 +282,9 @@ val type_inst_empty = store_thm(
     (!ta. temparg_inst empty_inst ta = SOME ta) /\
     (!tva. temp_valarg_inst empty_inst tva = SOME tva) /\
     (!sfld. sfld_inst empty_inst sfld = SOME sfld)``,
-  Q_TAC SUFF_TAC
-   `(!s ty. (s = empty_inst) ==> (type_inst s ty = SOME ty)) /\
-    (!s id. (s = empty_inst) ==> (cppid_inst s id = SOME (TypeID id))) /\
-    (!s ta. (s = empty_inst) ==> (temparg_inst s ta = SOME ta)) /\
-    (!s tva. (s = empty_inst) ==> (temp_valarg_inst s tva = SOME tva)) /\
-    (!s sfld. (s = empty_inst) ==> (sfld_inst s sfld = SOME sfld))`
-   THEN1 METIS_TAC [] THEN
   HO_MATCH_MP_TAC type_inst_ind THEN
-  SRW_TAC [][] THEN SRW_TAC [][] THENL [
-    Induct_on `tylist` THEN SRW_TAC [][empty_inst_def],
-    SRW_TAC [][empty_inst_def],
-    FULL_SIMP_TAC (srw_ss() ++ ETA_ss) [] THEN
-    `olmap (sfld_inst empty_inst) sfs = SOME sfs`
-       by (Induct_on `sfs` THEN SRW_TAC [][]) THEN
-    SRW_TAC [][],
-    SRW_TAC [][empty_inst_def],
-    SRW_TAC [ETA_ss] [] THEN Induct_on `targs` THEN SRW_TAC [][]
-  ]);
+  SRW_TAC [][] THEN SRW_TAC [][olmap_ALL_MEM, rich_listTheory.EL_IS_EL] THEN 
+  SRW_TAC [][empty_inst_def]);
 
 val type_match_refl = store_thm(
   "type_match_refl",
@@ -177,53 +297,92 @@ val cppID_inst_def = Define`
     case cppid_inst s id of NONE -> NONE || SOME ty -> typeid ty
 `;
 
+val tempmap_comp_def = Define`
+  tempmap_comp sigma (b,sfs,sn) = 
+    case sfs of 
+       [] -> if b then (T, [], sn) else sigma.tempmap sn
+    || h::t -> if b then (T, THE (olmap (sfld_inst sigma) sfs), sn) 
+               else 
+                 let sfs' = THE (olmap (sfld_inst sigma) sfs)
+                 in
+                   case typeid (THE (IDhd_inst 
+                                       sigma 
+                                       (F, THE (olmap (sfld_inst sigma) sfs), 
+                                        SFName sn)))
+                    of 
+                      SOME (IDConstant(b',sfs',SFName sn')) -> 
+                        (b',sfs',sn')
+                   || _ -> ARB
+`;
+
 val inst_comp_def = Define`
   inst_comp i2 i1 = <| typemap := THE o type_inst i2 o i1.typemap ;
-                       tempmap := THE o cppID_inst i2 o i1.tempmap ;
+                       tempmap := tempmap_comp i2 o i1.tempmap ;
                        valmap  := THE o temp_valarg_inst i2 o i1.valmap |>
 `;
 
 fun FTRY tac = TRY (tac THEN NO_TAC)
 
+val option_case_NONE2 = store_thm(
+  "option_case_NONE2", 
+  ``(option_case NONE (\x. NONE) y = NONE)``,
+  Cases_on `y` THEN SRW_TAC [][]);
+val _ = export_rewrites ["option_case_NONE2"]
+
 val cppid_non_typeid = store_thm(
   "cppid_non_typeid",
   ``(cppid_inst s id = SOME ty) /\ (typeid ty = NONE) ==>
-    ?nm. (id = IDVar nm) /\ (s.typemap nm = ty)``,
-  Cases_on `id` THEN SRW_TAC [][] THEN
-  Cases_on `p` THEN Cases_on `r` THEN SRW_TAC [][] THEN
-  Cases_on `typeid ty = NONE` THEN SRW_TAC [][] THEN
-  Cases_on `olmap (\a. sfld_inst s a) q'`  THEN SRW_TAC [][] THEN
-  Cases_on `sfld_inst s r'` THEN SRW_TAC [][] THEN
-  Cases_on `x = sfs'` THEN SRW_TAC [][] THEN
-  STRIP_TAC THEN SRW_TAC [][] THEN FULL_SIMP_TAC (srw_ss()) []);
+    ?nm. (id = IDConstant(F,[],SFName nm)) /\ (s.typemap nm = ty)``,
+  IDC_TAC `id` THEN SRW_TAC [][] THENL [
+    Cases_on `b` THEN Cases_on `sfs` THEN FSRW_TAC [IDhd_inst_EQ_SOME] THEN 
+    SRW_TAC [][] THEN FSRW_TAC [] THEN Cases_on `sf` THEN FSRW_TAC [],
+        
+    Cases_on `ty` THEN SRW_TAC [][]
+  ]);
 
-val option_case_EQ_SOME = store_thm(
-  "option_case_EQ_SOME",
-  ``(option_case NONE f v = SOME v0) =
-        ?v0'. (v = SOME v0') /\ (f v0' = SOME v0)``,
-  Cases_on `v` THEN SRW_TAC [][]);
-val _ = export_rewrites ["option_case_EQ_SOME"]
+val olmap_APPEND = store_thm(
+  "olmap_APPEND",
+  ``olmap f (l1 ++ l2) = 
+      case olmap f l1 of 
+         NONE -> NONE
+      || SOME l1' -> case olmap f l2 of 
+                        NONE -> NONE
+                     || SOME l2' -> SOME (l1' ++ l2')``,
+  Q.ID_SPEC_TAC `l2` THEN Induct_on`l1` THEN SRW_TAC [][] THENL [
+    Cases_on `olmap f l2` THEN SRW_TAC [][],
+    Cases_on `f h` THEN SRW_TAC [][] THEN 
+    Cases_on `olmap f l1` THEN SRW_TAC [][] THEN 
+    Cases_on `olmap f l2` THEN SRW_TAC [][]
+  ]);
 
+val SNOC_11 = store_thm(
+  "SNOC_11",
+  ``!x y l1 l2. (l1 ++ [x] = l2 ++ [y]) = (l1 = l2) /\ (x = y)``,
+  Induct_on `l1` THEN SRW_TAC [][] THENL [
+    Cases_on `l2` THEN SRW_TAC [][],
+    Cases_on `l2` THEN SRW_TAC [][] THEN METIS_TAC []
+  ]);
+    
 val inst_comp_thm = store_thm(
   "inst_comp_thm",
-  ``(!s1 ty1 ty2 ty3 s2.
+  ``(!ty1 s1 ty2 ty3 s2.
         (type_inst s1 ty1 = SOME ty2) /\
         (type_inst s2 ty2 = SOME ty3) ==>
         (type_inst (inst_comp s2 s1) ty1 = SOME ty3)) /\
-    (!s1 id1 s2 ty2 id3 ty4.
+    (!id1 s1 s2 ty2 id3 ty4.
         (cppid_inst s1 id1 = SOME ty2) /\
         (typeid ty2 = SOME id3) /\
         (cppid_inst s2 id3 = SOME ty4) ==>
         (cppid_inst (inst_comp s2 s1) id1 = SOME ty4)) /\
-    (!s1 ta1 ta2 ta3 s2.
+    (!ta1 s1 ta2 ta3 s2.
         (temparg_inst s1 ta1 = SOME ta2) /\
         (temparg_inst s2 ta2 = SOME ta3) ==>
         (temparg_inst (inst_comp s2 s1) ta1 = SOME ta3)) /\
-    (!s1 tva1 tva2 tva3 s2.
+    (!tva1 s1 tva2 tva3 s2.
         (temp_valarg_inst s1 tva1 = SOME tva2) /\
         (temp_valarg_inst s2 tva2 = SOME tva3) ==>
         (temp_valarg_inst (inst_comp s2 s1) tva1 = SOME tva3)) /\
-    (!s1 sfld1 sfld2 sfld3 s2.
+    (!sfld1 s1 sfld2 sfld3 s2.
         (sfld_inst s1 sfld1 = SOME sfld2) /\
         (sfld_inst s2 sfld2 = SOME sfld3) ==>
         (sfld_inst (inst_comp s2 s1) sfld1 = SOME sfld3))``,
@@ -232,164 +391,199 @@ val inst_comp_thm = store_thm(
   FTRY (FULL_SIMP_TAC (srw_ss()) []) THENL [
     (* TypeID *)
     Cases_on `typeid ty2` THENL [
-      `?nm. (id1 = IDVar nm) /\ (s1.typemap nm = ty2)`
+      `?nm. (id1 = IDConstant (F, [], SFName nm)) /\ (s1.typemap nm = ty2)`
          by METIS_TAC [cppid_non_typeid] THEN
-      SRW_TAC [][inst_comp_def],
-      `ty2 = TypeID x`
-         by (Cases_on `ty2` THEN FULL_SIMP_TAC (srw_ss()) []) THEN
-      FULL_SIMP_TAC (srw_ss()) []
+      SRW_TAC [][inst_comp_def, IDhd_inst_def],
+      `ty2 = TypeID x` by (Cases_on `ty2` THEN FSRW_TAC []) THEN
+      FSRW_TAC []
     ],
 
     (* MPtr *)
-    FULL_SIMP_TAC (srw_ss()) [] THEN PROVE_TAC [],
+    FSRW_TAC [] THEN PROVE_TAC [],
 
     (* Function (type) case *)
-    FULL_SIMP_TAC (srw_ss() ++ ETA_ss) [] THEN
-    Induct_on `tylist` THEN SRW_TAC [][] THENL [
-      FULL_SIMP_TAC (srw_ss()) [],
-      FULL_SIMP_TAC (srw_ss()) [DISJ_IMP_THM, FORALL_AND_THM]
+    FSRW_TAC [olmap_ALL_MEM] THEN REPEAT STRIP_TAC THEN 
+    Q_TAC SUFF_TAC `MEM (EL i tylist) tylist /\
+                    ?ty2. (type_inst s1 (EL i tylist) = SOME ty2) /\
+                          (type_inst s2 ty2 = SOME (EL i y0'))`
+          THEN1 METIS_TAC [] THEN 
+    SRW_TAC [][rich_listTheory.EL_IS_EL],
 
+    (* IDVar case ? *)
+    FSRW_TAC [] THEN SRW_TAC [][] THEN FSRW_TAC [],
 
-SRW_TAC [][] THEN
-  FTRY (SRW_TAC [][]) THEN FTRY (FULL_SIMP_TAC (srw_ss()) []) THEN
-  FTRY (RES_TAC THEN SRW_TAC [][])
+    (* IDConstant case 1 *)
+    FSRW_TAC [] THEN SRW_TAC [][] THEN FSRW_TAC [] THEN SRW_TAC [][] THEN 
+    FSRW_TAC [olmap_ALL_MEM] THEN SRW_TAC [][] THEN 
+    RULE_ASSUM_TAC (SIMP_RULE (bool_ss ++ DNF_ss) [AND_IMP_INTRO]) THEN 
+    FIRST_X_ASSUM MATCH_MP_TAC THEN SRW_TAC [][rich_listTheory.EL_IS_EL],
 
-    (!ty1 ty2 ty3 s1 s2.
-    (!p1 p2 p3 s1 s2 b1 b2 b3
+    (* IDConstant case 2 *)
+    FSRW_TAC [IDhd_inst_EQ_SOME] THEN SRW_TAC [][] THEN FSRW_TAC [] THENL [
+      FSRW_TAC [olmap_EQ_SOME] THEN SRW_TAC [][] THEN 
+      Q.EXISTS_TAC `SFName s'` THEN SRW_TAC [][] THEN 
+      SRW_TAC [][inst_comp_def] THEN 
+      Cases_on `s1.typemap s'` THEN FSRW_TAC [],
 
-    (!tal1 tal2 tal3 s1 s2.
-        (olmap (temparg_inst s1) tal1 = SOME tal2) /\
-        (olmap (temparg_inst s2) tal2 = SOME tal3) ==>
-        (olmap (temparg_inst (inst_comp s2 s1)) tal1 = SOME tal3)) /\
-    (!tyl1 tyl2 tyl3 s1 s2.
-        (olmap (type_inst s1) tyl1 = SOME tyl2) /\
-        (olmap (type_inst s2) tyl2 = SOME tyl3) ==>
-        (olmap (type_inst (inst_comp s2 s1)) tyl1 = SOME tyl3)) /\
-    (!sflist1 sflist2 sflist3 s1 s2.
-        (olmap (sfld_inst s1) sflist1 = SOME sflist2) /\
-        (olmap (sfld_inst s2) sflist2 = SOME sflist3) ==>
-        (olmap (sfld_inst (inst_comp s2 s1)) sflist1 = SOME sflist3))``,
-  Induct THEN SRW_TAC [][] THEN
-  FTRY (SRW_TAC[][]) THEN FTRY (FULL_SIMP_TAC (srw_ss()) []) THEN
-  FTRY (RES_TAC THEN SRW_TAC [][]) THENL [
-    (* IDVar case *)
-    Cases_on `s1.typemap s` THEN FULL_SIMP_TAC (srw_ss()) [] THEN
+      SRW_TAC [][] THEN FSRW_TAC [olmap_EQ_SOME] THEN SRW_TAC [][] THEN 
+      Cases_on `b2` THENL [
+        FSRW_TAC [] THEN SRW_TAC [][] THEN 
+        Q.EXISTS_TAC `SFTempCall s' z` THEN SRW_TAC [][] THEN 
+        SRW_TAC [][inst_comp_def, tempmap_comp_def] THEN 
+        Cases_on `sfs2` THEN FULL_SIMP_TAC (srw_ss() ++ ETA_ss) [],
+        FSRW_TAC [] THEN SRW_TAC [][] THEN 
+        FSRW_TAC [IDhd_inst_EQ_SOME] THEN SRW_TAC [][] THENL [
+          FULL_SIMP_TAC (srw_ss() ++ ETA_ss) [olmap_EQ_SOME] THEN 
+          SRW_TAC [][] THEN Q.EXISTS_TAC `SFTempCall s' z` THEN 
+          SRW_TAC [][] THENL [
+            FIRST_X_ASSUM MATCH_MP_TAC THEN 
+            Q.EXISTS_TAC `SFTempCall s' tas` THEN 
+            SRW_TAC [ETA_ss][],
+            SRW_TAC [][inst_comp_def, tempmap_comp_def]
+          ],
+          Q.EXISTS_TAC `SFTempCall s' z` THEN SRW_TAC [][] THEN 
+          FSRW_TAC [olmap_EQ_SOME] THEN SRW_TAC [][] THEN 
+          FULL_SIMP_TAC (srw_ss() ++ ETA_ss) [] THEN 
+          SRW_TAC [][inst_comp_def, tempmap_comp_def] THEN 
+          Q.UNABBREV_ALL_TAC THEN SRW_TAC [][IDhd_inst_def],
+          FULL_SIMP_TAC (srw_ss() ++ ETA_ss) [olmap_EQ_SOME] THEN 
+          SRW_TAC [][] THEN Q.EXISTS_TAC `SFTempCall s' z` THEN 
+          SRW_TAC [][] THENL [
+            FIRST_X_ASSUM MATCH_MP_TAC THEN 
+            Q.EXISTS_TAC `SFTempCall s' tas` THEN 
+            SRW_TAC [ETA_ss][],
+            SRW_TAC [][inst_comp_def, tempmap_comp_def] THEN 
+            Q.UNABBREV_ALL_TAC THEN SRW_TAC [][IDhd_inst_def]
+          ]
+        ]
+      ],
+
+      SRW_TAC [][] THEN 
+      FULL_SIMP_TAC (srw_ss() ++ ETA_ss) [olmap_EQ_SOME] THEN SRW_TAC [][] THEN
+      Cases_on `a` THEN FSRW_TAC [] THEN SRW_TAC [][] THEN 
+      SRW_TAC [DNF_ss][] THEN Cases_on `b'` THEN FSRW_TAC [] THENL [
+        SRW_TAC [][] THEN SRW_TAC [DNF_ss][] THEN 
+        FULL_SIMP_TAC (srw_ss() ++ ETA_ss) [olmap_APPEND] THEN 
+        SRW_TAC [][] THEN 
+        MAP_EVERY Q.EXISTS_TAC [`l2''`, `l1''`, `h`] THEN 
+        SRW_TAC [][] THENL [ 
+          FULL_SIMP_TAC (srw_ss() ++ DNF_ss) [AND_IMP_INTRO, olmap_ALL_MEM] THEN
+          SRW_TAC [][] THEN FIRST_X_ASSUM MATCH_MP_TAC THEN 
+          METIS_TAC [rich_listTheory.EL_IS_EL],
+          SRW_TAC [ETA_ss][inst_comp_def]
+        ],
+        FULL_SIMP_TAC (srw_ss() ++ ETA_ss) [olmap_APPEND] THEN SRW_TAC [][] THEN
+        MAP_EVERY Q.EXISTS_TAC [`l2''`,`sf'''`] THEN SRW_TAC [][] THEN 
+        FULL_SIMP_TAC (srw_ss() ++ DNF_ss)
+                      [IDhd_inst_EQ_SOME, AND_IMP_INTRO] 
+        THENL [
+          SRW_TAC [][] THEN Cases_on `l1''` THENL [
+            FSRW_TAC [] THEN SRW_TAC [][] THEN 
+            FSRW_TAC [olmap_EQ_SOME] THEN SRW_TAC [][] THEN 
+            MAP_EVERY Q.EXISTS_TAC [`sfs1'`, `sf1'`] THEN 
+            SRW_TAC [][] THENL [
+              FSRW_TAC [olmap_ALL_MEM] THEN SRW_TAC [][] THEN 
+              FIRST_X_ASSUM MATCH_MP_TAC THEN 
+              METIS_TAC [rich_listTheory.EL_IS_EL],
+              SRW_TAC [][inst_comp_def, IDhd_inst_def]
+            ],
+            FSRW_TAC [] THEN SRW_TAC [][] THEN 
+            FSRW_TAC [olmap_EQ_SOME] THEN SRW_TAC [][] THEN 
+            MAP_EVERY Q.EXISTS_TAC [`sfs1' ++ [sf1'] ++ t`, `h`] THEN 
+            SRW_TAC [][] THENL [
+              FSRW_TAC [olmap_ALL_MEM] THEN SRW_TAC [][] THEN 
+              METIS_TAC [rich_listTheory.EL_IS_EL],
+              SRW_TAC [ETA_ss][inst_comp_def, IDhd_inst_def]
+            ]
+          ],
+          SRW_TAC [][] THEN Cases_on `l1''` THENL [
+            FSRW_TAC [] THEN SRW_TAC [][] THEN 
+            FSRW_TAC [olmap_EQ_SOME] THEN SRW_TAC [][] THEN 
+            SRW_TAC [][SNOC_11] THENL [
+              FSRW_TAC [olmap_ALL_MEM] THEN SRW_TAC [][] THEN 
+              METIS_TAC [rich_listTheory.EL_IS_EL],
+              SRW_TAC [ETA_ss][inst_comp_def, IDhd_inst_def]
+            ],
+            FSRW_TAC [] THEN SRW_TAC [][] THEN 
+            FSRW_TAC [olmap_EQ_SOME] THEN SRW_TAC [][] THEN 
+            REWRITE_TAC [SNOC_11] THEN SRW_TAC [][] THENL [
+              FSRW_TAC [olmap_ALL_MEM] THEN SRW_TAC [][] THEN 
+              METIS_TAC [rich_listTheory.EL_IS_EL],
+              SRW_TAC [ETA_ss][inst_comp_def, IDhd_inst_def]
+            ]
+          ]
+        ]
+      ],
+
+      SRW_TAC [][] THEN 
+      FULL_SIMP_TAC (srw_ss() ++ ETA_ss) [olmap_EQ_SOME] THEN 
+      SRW_TAC [][] THEN SRW_TAC [DNF_ss][] THEN 
+      Cases_on `b2` THEN FSRW_TAC [] THENL [
+        SRW_TAC [][] THEN 
+        FULL_SIMP_TAC (srw_ss() ++ ETA_ss) [olmap_APPEND] THEN 
+        SRW_TAC [][] THEN DISJ2_TAC THEN 
+        MAP_EVERY Q.EXISTS_TAC [`l2''`, `s'`, `z`, `l1''`, `sfn2`] THEN 
+        SRW_TAC [][] THENL [
+          Cases_on `a` THEN FSRW_TAC [] THEN SRW_TAC [ETA_ss][] THEN 
+          FULL_SIMP_TAC (srw_ss() ++ DNF_ss ++ ETA_ss) [],
+          FULL_SIMP_TAC (srw_ss() ++ DNF_ss ++ ETA_ss) [olmap_ALL_MEM] THEN 
+          METIS_TAC [rich_listTheory.EL_IS_EL],
+          SRW_TAC [][inst_comp_def, tempmap_comp_def] THEN 
+          Cases_on `sfs1` THEN SRW_TAC [][] THEN 
+          FSRW_TAC [olmap_EQ_SOME]
+        ],
+        Cases_on `a` THEN FSRW_TAC [] THEN SRW_TAC [][] THEN 
+        FULL_SIMP_TAC (srw_ss() ++ ETA_ss) [olmap_APPEND] THEN 
+        SRW_TAC [][] THEN FSRW_TAC [IDhd_inst_EQ_SOME] THENL [
+          Q.EXISTS_TAC `l2''` THEN 
+          Cases_on `l1''` THEN FSRW_TAC [] THEN SRW_TAC [][] THEN 
+          SRW_TAC [][SNOC_11] THENL [
+            FULL_SIMP_TAC (srw_ss() ++ DNF_ss ++ ETA_ss) [],
+            FSRW_TAC [olmap_ALL_MEM] THEN METIS_TAC [rich_listTheory.EL_IS_EL],
+            SRW_TAC [][inst_comp_def, tempmap_comp_def] THEN 
+            FSRW_TAC [olmap_EQ_SOME] THEN 
+            SRW_TAC [][LET_THM, IDhd_inst_def]
+          ],
+          SRW_TAC [][] THEN Q.EXISTS_TAC `l2''` THEN 
+          Cases_on `l1''` THENL [
+            FSRW_TAC [olmap_EQ_SOME] THEN SRW_TAC [][SNOC_11] THENL [
+              FULL_SIMP_TAC (srw_ss() ++ DNF_ss ++ ETA_ss) [],
+              FSRW_TAC [olmap_ALL_MEM] THEN 
+              METIS_TAC [rich_listTheory.EL_IS_EL],
+              SRW_TAC [][inst_comp_def, tempmap_comp_def]
+            ],
+            FSRW_TAC [olmap_EQ_SOME] THEN SRW_TAC [][SNOC_11] THENL [
+              FULL_SIMP_TAC (srw_ss() ++ DNF_ss ++ ETA_ss) [],
+              FSRW_TAC [olmap_ALL_MEM] THEN 
+              METIS_TAC [rich_listTheory.EL_IS_EL],
+              SRW_TAC [][inst_comp_def, tempmap_comp_def, LET_THM, 
+                         IDhd_inst_def]
+            ]
+          ]
+        ]
+      ]
+    ],
+
+    (* TTemp case *)
+    FULL_SIMP_TAC (srw_ss()) [] THEN SRW_TAC [][] THEN METIS_TAC [],
+
+    (* TOBj case *)
+    FULL_SIMP_TAC (srw_ss()) [] THEN SRW_TAC [][] THEN METIS_TAC [],
+
+    (* TMPtr case *) 
+    FULL_SIMP_TAC (srw_ss()) [] THEN SRW_TAC [][] THEN 
+    Q.EXISTS_TAC `ty'` THEN SRW_TAC [][],
+
+    (* some tva case *)
+    Cases_on `s1.valmap s` THEN FULL_SIMP_TAC (srw_ss()) [] THEN 
     SRW_TAC [][inst_comp_def],
 
-    (* IDConstant *)
-    Cases_on `p` THEN Cases_on `r` THEN
-    FULL_SIMP_TAC (srw_ss()) [] THEN SRW_TAC [][] THEN
-    FULL_SIMP_TAC (srw_ss()) [] THEN SRW_TAC [][] THEN
-    FULL_SIMP_TAC (srw_ss()) [] THEN SRW_TAC [][] THEN
-    SRW_TAC [ETA_ss][inst_comp_def]
-
-    (* SFTempCall *)
-    FULL_SIMP_TAC (srw_ss() ++ ETA_ss) [],
-
-    (* TObj *)
-    FULL_SIMP_TAC (srw_ss()) [] THEN PROVE_TAC [],
-
-    (* TMPtr *)
-    FULL_SIMP_TAC (srw_ss()) [] THEN SRW_TAC [][] THEN PROVE_TAC [],
-
-    (* TVAVar *)
-    SRW_TAC [][inst_comp_def],
-
-    (* MPtr *)
-    FULL_SIMP_TAC (srw_ss()) [] THEN PROVE_TAC [],
-
-    (* Function (type) case *)
-    FULL_SIMP_TAC (srw_ss() ++ ETA_ss) [],
-
-    (* typeid case (?) *)
-    Cases_on `typeid ty2` THENL [
-      `?nm. (id1 = IDVar nm) /\ (s1.typemap nm = ty2)`
-          by METIS_TAC [cppid_non_typeid] THEN
-      SRW_TAC [][inst_comp_def],
-      `ty2 = TypeID x`
-         by (Cases_on `ty2` THEN FULL_SIMP_TAC (srw_ss()) []) THEN
-      FULL_SIMP_TAC (srw_ss()) []
-    ]
-  ]);
-
-val inst_comp_thm = store_thm(
-  "inst_comp_thm",
-  ``(!id1 s1 s2 ty2 id3 ty4.
-        (cppid_inst s1 id1 = SOME ty2) /\
-        (typeid ty2 = SOME id3) /\
-        (cppid_inst s2 id3 = SOME ty4) ==>
-        (cppid_inst (inst_comp s2 s1) id1 = SOME ty4)) /\
-    (!sfld1 sfld2 sfld3 s1 s2.
-        (sfld_inst s1 sfld1 = SOME sfld2) /\
-        (sfld_inst s2 sfld2 = SOME sfld3) ==>
-        (sfld_inst (inst_comp s2 s1) sfld1 = SOME sfld3)) /\
-    (!ta1 ta2 ta3 s1 s2.
-        (temparg_inst s1 ta1 = SOME ta2) /\
-        (temparg_inst s2 ta2 = SOME ta3) ==>
-        (temparg_inst (inst_comp s2 s1) ta1 = SOME ta3)) /\
-    (!tva1 tva2 tva3 s1 s2.
-        (temp_valarg_inst s1 tva1 = SOME tva2) /\
-        (temp_valarg_inst s2 tva2 = SOME tva3) ==>
-        (temp_valarg_inst (inst_comp s2 s1) tva1 = SOME tva3)) /\
-    (!ty1 ty2 ty3 s1 s2.
-        (type_inst s1 ty1 = SOME ty2) /\
-        (type_inst s2 ty2 = SOME ty3) ==>
-        (type_inst (inst_comp s2 s1) ty1 = SOME ty3)) /\
-    (!p1 p2 p3 s1 s2 b1 b2 b3
-
-    (!tal1 tal2 tal3 s1 s2.
-        (olmap (temparg_inst s1) tal1 = SOME tal2) /\
-        (olmap (temparg_inst s2) tal2 = SOME tal3) ==>
-        (olmap (temparg_inst (inst_comp s2 s1)) tal1 = SOME tal3)) /\
-    (!tyl1 tyl2 tyl3 s1 s2.
-        (olmap (type_inst s1) tyl1 = SOME tyl2) /\
-        (olmap (type_inst s2) tyl2 = SOME tyl3) ==>
-        (olmap (type_inst (inst_comp s2 s1)) tyl1 = SOME tyl3)) /\
-    (!sflist1 sflist2 sflist3 s1 s2.
-        (olmap (sfld_inst s1) sflist1 = SOME sflist2) /\
-        (olmap (sfld_inst s2) sflist2 = SOME sflist3) ==>
-        (olmap (sfld_inst (inst_comp s2 s1)) sflist1 = SOME sflist3))``,
-  Induct THEN SRW_TAC [][] THEN
-  FTRY (SRW_TAC[][]) THEN FTRY (FULL_SIMP_TAC (srw_ss()) []) THEN
-  FTRY (RES_TAC THEN SRW_TAC [][]) THENL [
-    (* IDVar case *)
-    Cases_on `s1.typemap s` THEN FULL_SIMP_TAC (srw_ss()) [] THEN
-    SRW_TAC [][inst_comp_def],
-
-    (* IDConstant *)
-    Cases_on `p` THEN Cases_on `r` THEN
-    FULL_SIMP_TAC (srw_ss()) [] THEN SRW_TAC [][] THEN
-    FULL_SIMP_TAC (srw_ss()) [] THEN SRW_TAC [][] THEN
-    FULL_SIMP_TAC (srw_ss()) [] THEN SRW_TAC [][] THEN
-    SRW_TAC [ETA_ss][inst_comp_def]
-
-    (* SFTempCall *)
-    FULL_SIMP_TAC (srw_ss() ++ ETA_ss) [],
-
-    (* TObj *)
-    FULL_SIMP_TAC (srw_ss()) [] THEN PROVE_TAC [],
-
-    (* TMPtr *)
-    FULL_SIMP_TAC (srw_ss()) [] THEN SRW_TAC [][] THEN PROVE_TAC [],
-
-    (* TVAVar *)
-    SRW_TAC [][inst_comp_def],
-
-    (* MPtr *)
-    FULL_SIMP_TAC (srw_ss()) [] THEN PROVE_TAC [],
-
-    (* Function (type) case *)
-    FULL_SIMP_TAC (srw_ss() ++ ETA_ss) [],
-
-    (* typeid case (?) *)
-    Cases_on `typeid ty2` THENL [
-      `?nm. (id1 = IDVar nm) /\ (s1.typemap nm = ty2)`
-          by METIS_TAC [cppid_non_typeid] THEN
-      SRW_TAC [][inst_comp_def],
-      `ty2 = TypeID x`
-         by (Cases_on `ty2` THEN FULL_SIMP_TAC (srw_ss()) []) THEN
-      FULL_SIMP_TAC (srw_ss()) []
-    ]
+    (* SFTEmpCall case *)
+    FULL_SIMP_TAC (srw_ss()) [] THEN SRW_TAC [][] THEN 
+    FULL_SIMP_TAC (srw_ss() ++ ETA_ss) [olmap_ALL_MEM] THEN 
+    RULE_ASSUM_TAC (SIMP_RULE (bool_ss ++ DNF_ss) [AND_IMP_INTRO]) THEN 
+    SRW_TAC [][] THEN FIRST_X_ASSUM MATCH_MP_TAC THEN 
+    SRW_TAC [][rich_listTheory.EL_IS_EL]
   ]);
 
 (* SANITY theorem = comment under definition 2 to the effect <= is
@@ -401,9 +595,10 @@ val type_match_trans = store_thm(
   SRW_TAC [][inst_comp_thm]);
 
 val is_renaming_def = Define`
-  is_renaming s = (!v. ?nm. s.typemap v = TypeID (IDVar nm)) /\
-                  (!v. ?nm. s.tempmap v = TemplateVar nm) /\
-                  (!v. ?nm. s.valmap v = TVAVar nm)
+  is_renaming s = 
+    (!v. ?nm. s.typemap v = TypeID (IDConstant(F,[],SFName nm))) /\
+    (!v. ?nm. s.tempmap v = (F,[],nm)) /\
+    (!v. ?nm. s.valmap v = TVAVar nm)
 `;
 
 val empty_inst_is_renaming = store_thm(
@@ -411,26 +606,15 @@ val empty_inst_is_renaming = store_thm(
   ``is_renaming empty_inst``,
   SRW_TAC [][empty_inst_def, is_renaming_def]);
 
-val tidinst_sz_def = Define`
-  (tidinst_sz (TemplateConstant n) = 1n) /\
-  (tidinst_sz (TemplateVar s) = 0)
-`;
-val _ = export_rewrites ["tidinst_sz_def"]
-
-val tempid_inst_size = store_thm(
-  "tempid_inst_size",
-  ``tidinst_sz tid <= tidinst_sz (tempid_inst s tid)``,
-  Cases_on `tid` THEN SRW_TAC [][]);
-
 val tyinst_sz_def = Define`
-  (tyinst_sz (Class cid) = 2) /\
+  (tyinst_sz (Class cid) = 2n) /\
   (tyinst_sz (Ptr ty) = 1 + tyinst_sz ty) /\
   (tyinst_sz (MPtr id ty) = 1 + cppidinst_sz id + tyinst_sz ty) /\
   (tyinst_sz (Ref ty) = 1 + tyinst_sz ty) /\
   (tyinst_sz (Array ty n) = 1 + tyinst_sz ty) /\
   (tyinst_sz (Function ty tyl) = 1 + tyinst_sz ty + tylinst_sz tyl) /\
   (tyinst_sz (Const ty) = 1 + tyinst_sz ty) /\
-  (tyinst_sz (TypeID id) = 1 + cppidinst_sz id) /\
+  (tyinst_sz (TypeID id) = 1) /\
   (tyinst_sz Void = 2) /\
   (tyinst_sz BChar = 2) /\
   (tyinst_sz Bool = 2) /\
@@ -442,10 +626,7 @@ val tyinst_sz_def = Define`
 
      /\
 
-  (cppidinst_sz (IDVar s) = 0) /\
-  (cppidinst_sz (IDFld id sfld) = cppidinst_sz id + sfldinst_sz sfld + 1) /\
-  (cppidinst_sz (IDTempCall tid tal) =
-     tidinst_sz tid + talinst_sz tal + 1) /\
+  (cppidinst_sz (IDVar s) = 1) /\
   (cppidinst_sz (IDConstant tn) = 1)
 
      /\
@@ -456,7 +637,7 @@ val tyinst_sz_def = Define`
      /\
 
   (tainst_sz (TType ty) = 1 + tyinst_sz ty) /\
-  (tainst_sz (TTemp tid) = 1 + tidinst_sz tid) /\
+  (tainst_sz (TTemp tid) = 1 + cppidinst_sz tid) /\
   (tainst_sz (TVal tva) = 1 + tvainst_sz tva)
 
      /\
@@ -480,7 +661,7 @@ val _ = export_rewrites ["tyinst_sz_def"]
 
 val typeid_size = store_thm(
   "typeid_size",
-  ``(typeid ty = SOME id) ==> (tyinst_sz ty = 1 + cppidinst_sz id)``,
+  ``(typeid ty = SOME id) ==> (tyinst_sz ty = 1)``,
   Cases_on `ty` THEN SRW_TAC [][]);
 
 val zero_lt_tysize = store_thm(
@@ -488,15 +669,9 @@ val zero_lt_tysize = store_thm(
   ``0 < tyinst_sz ty``,
   Cases_on `ty` THEN SRW_TAC [ARITH_ss][]);
 
-val cppidinst_sz_EQ_0 = store_thm(
-  "cppidinst_sz_EQ_0",
-  ``(cppidinst_sz id = 0) = ?nm. id = IDVar nm``,
-  Cases_on `id` THEN SRW_TAC [][]);
-val _ = export_rewrites ["cppidinst_sz_EQ_0"]
-
 val tyinst_sz_EQ_1 = store_thm(
   "tyinst_sz_EQ_1",
-  ``(tyinst_sz ty = 1) = ?nm. ty = TypeID (IDVar nm)``,
+  ``(tyinst_sz ty = 1) = ?id. ty = TypeID id``,
   Cases_on `ty` THEN SRW_TAC [][] THEN
   MP_TAC (Q.INST [`ty` |-> `C''`] zero_lt_tysize) THEN
   TRY DECIDE_TAC THEN
@@ -512,7 +687,7 @@ val _ = export_rewrites ["tvainst_sz_EQ_0"]
 val type_match_size_increase = store_thm(
   "type_match_size_increase",
   ``(!id1 s ty2. (cppid_inst s id1 = SOME ty2) ==>
-                 cppidinst_sz id1 < tyinst_sz ty2) /\
+                 cppidinst_sz id1 <= tyinst_sz ty2) /\
     (!sfld1 s sfld2. (sfld_inst s sfld1 = SOME sfld2) ==>
                      sfldinst_sz sfld1 <= sfldinst_sz sfld2) /\
     (!ta1 s ta2. (temparg_inst s ta1 = SOME ta2) ==>
@@ -528,19 +703,23 @@ val type_match_size_increase = store_thm(
   Induct THEN SRW_TAC [][] THEN SRW_TAC [][] THEN
   FTRY (RES_TAC THEN DECIDE_TAC) THEN
   FTRY (IMP_RES_TAC typeid_size THEN RES_TAC THEN DECIDE_TAC) THENL [
+    Cases_on `p` THEN Case
     MATCH_ACCEPT_TAC (GEN_ALL zero_lt_tysize),
 
-    FULL_SIMP_TAC (srw_ss() ++ ETA_ss) [] THEN RES_TAC THEN
-    MP_TAC (Q.INST [`tid` |-> `T'`] tempid_inst_size) THEN
-    DECIDE_TAC,
+    Cases_on `p` THEN Cases_on `r` THEN Cases_on `q` THEN 
+    FULL_SIMP_TAC (srw_ss()) [] THEN SRW_TAC [][] THEN 
+    FSRW_TAC [IDhd_inst_EQ_SOME] THEN SRW_TAC [][] THEN 
+    Cases_on `s.typemap s'` THEN SRW_TAC [ARITH_ss][zero_lt_tysize] THENL [
+      Q.SPEC_THEN `C0` MP_TAC (GEN_ALL zero_lt_tysize) THEN DECIDE_TAC,
+      Q.SPEC_THEN `C''` MP_TAC (GEN_ALL zero_lt_tysize) THEN DECIDE_TAC,
+      
+      
+    
 
-    FULL_SIMP_TAC (srw_ss() ++ ETA_ss) [] THEN RES_TAC THEN DECIDE_TAC,
-
-    SRW_TAC [][tempid_inst_size],
+    FULL_SIMP_TAC (srw_ss() ++ ETA_ss) [] THEN RES_TAC,
 
     FULL_SIMP_TAC (srw_ss() ++ ETA_ss) [] THEN RES_TAC THEN DECIDE_TAC
   ]);
-
 val _ = Hol_datatype`frees_record = <| tyfvs : string set ;
                                        tempfvs : string set ;
                                        valfvs : string set |>`
@@ -571,7 +750,7 @@ val renaming_upto_def = Define`
   renaming_upto frees s = (!v. v IN frees.tyfvs ==>
                                ?nm. s.typemap v = TypeID (IDVar nm)) /\
                           (!v. v IN frees.tempfvs ==>
-                               ?nm. s.tempmap v = TemplateVar nm) /\
+                               ?nm. s.tempmap v = IDVar nm) /\
                           (!v. v IN frees.valfvs ==>
                                ?nm. s.valmap v = TVAVar nm)
 `;
@@ -589,20 +768,14 @@ val renaming_upto_UNION = store_thm(
   METIS_TAC []);
 val _ = export_rewrites ["renaming_upto_UNION"]
 
-val tidfrees_def = Define`
-  (tidfrees (TemplateConstant tn) = {}) /\
-  (tidfrees (TemplateVar s) = tempfree_sing s)
-`;
-val _ = export_rewrites ["tidfrees_def"]
-
-
-val tyfrees_def = Define`
+val tyfrees_defn = Defn.Hol_defn "tyfrees" `
   (tyfrees (Class cid) = {}) /\
   (tyfrees (Ptr ty) = tyfrees ty) /\
   (tyfrees (MPtr id ty) = cppidfrees id UNION tyfrees ty) /\
   (tyfrees (Ref ty) = tyfrees ty) /\
   (tyfrees (Array ty n) = tyfrees ty) /\
-  (tyfrees (Function ty tyl) = tyfrees ty UNION tylfrees tyl) /\
+  (tyfrees (Function ty tyl) = 
+     FOLDL (\a ty.  a UNION tyfrees ty) (tyfrees ty) tyl) /\
   (tyfrees (Const ty) = tyfrees ty) /\
   (tyfrees (TypeID id) = cppidfrees id) /\
   (tyfrees Void = {}) /\
@@ -617,19 +790,18 @@ val tyfrees_def = Define`
      /\
 
   (cppidfrees (IDVar s) = tyfree_sing s) /\
-  (cppidfrees (IDFld id sfld) = cppidfrees id UNION sfldfrees sfld) /\
-  (cppidfrees (IDTempCall tid tal) = tidfrees tid UNION talfrees tal) /\
-  (cppidfrees (IDConstant tn) = {})
+  (cppidfrees (IDConstant (b,sfs,sf)) = 
+     FOLDL (\a sf. a UNION sfldfrees sf) (sfldfrees sf) sfs)
 
      /\
 
-  (sfldfrees (SFTempCall s tal) = talfrees tal) /\
+  (sfldfrees (SFTempCall s tal) = FOLDL (\a ta. a UNION tafrees ta) {} tal) /\
   (sfldfrees (SFName s) = {})
 
      /\
 
   (tafrees (TType ty) = tyfrees ty) /\
-  (tafrees (TTemp tid) = tidfrees tid) /\
+  (tafrees (TTemp tid) = cppidfrees tid) /\
   (tafrees (TVal tva) = tvalfrees tva)
 
      /\
@@ -638,44 +810,102 @@ val tyfrees_def = Define`
   (tvalfrees (TObj id) = cppidfrees id) /\
   (tvalfrees (TMPtr id ty) = cppidfrees id UNION tyfrees ty) /\
   (tvalfrees (TVAVar s) = valfree_sing s)
-
-     /\
-
-  (talfrees [] = {}) /\
-  (talfrees (ta::tal) = tafrees ta UNION talfrees tal)
-
-     /\
-
-  (tylfrees [] = {}) /\
-  (tylfrees (ty::tyl) = tyfrees ty UNION tylfrees tyl)
 `
+
+val (tyfrees_def, tyfrees_ind) = Defn.tprove(
+  tyfrees_defn, 
+  WF_REL_TAC 
+    `^(last (TotalDefn.guessR tyfrees_defn))` THEN 
+  SRW_TAC [ARITH_ss][] THENL [
+    Induct_on `tyl` THEN SRW_TAC [][] THEN SRW_TAC [ARITH_ss][] THEN 
+    FULL_SIMP_TAC (srw_ss() ++ ARITH_ss) [],
+    Induct_on `sfs` THEN SRW_TAC [][] THEN 
+    FULL_SIMP_TAC (srw_ss() ++ ARITH_ss) [],
+    Induct_on `tal` THEN SRW_TAC [][] THEN 
+    FULL_SIMP_TAC (srw_ss() ++ ARITH_ss) []
+  ]);
+val _ = save_thm("tyfrees_def", tyfrees_def)
+val _ = save_thm("tyfrees_ind", tyfrees_ind)
 val _ = export_rewrites ["tyfrees_def"]
 
-val inst_size_tidrenaming = store_thm(
-  "inst_size_tidrenaming",
-  ``(tidinst_sz (tempid_inst s tid) = tidinst_sz tid) ==>
-    renaming_upto (tidfrees tid) s``,
-  Cases_on `tid` THEN SRW_TAC [][tempfree_sing_def] THEN
-  Cases_on `s.tempmap s'` THEN FULL_SIMP_TAC (srw_ss()) [] THEN
-  SRW_TAC [][renaming_upto_def]);
+val renaming_upto_FOLDL = store_thm(
+  "renaming_upto_FOLDL",
+  ``!list acc s. 
+       (!e. MEM e list ==> renaming_upto (f e) s) /\
+       renaming_upto acc s ==> 
+       renaming_upto (FOLDL (\a e. a UNION f e) acc list) s``,
+  Induct THEN SRW_TAC [][]);
 
+val tylinst_sz_leq = prove(
+  ``!xl yl x y. 
+      (x + tylinst_sz xl = y + tylinst_sz yl) /\ x <= y /\
+      (LENGTH xl = LENGTH yl) /\
+      (!i. i < LENGTH xl ==> tyinst_sz (EL i xl) <= tyinst_sz (EL i yl)) ==>
+      (x = y) /\ (tylinst_sz xl = tylinst_sz yl)``,
+  Induct THEN1 SRW_TAC [ARITH_ss][] THEN 
+  Cases_on `yl` THEN SIMP_TAC (srw_ss()) [] THEN 
+  REPEAT GEN_TAC THEN STRIP_TAC THEN
+  `tyinst_sz h' <= tyinst_sz h`
+      by (FIRST_X_ASSUM (Q.SPEC_THEN `0` MP_TAC) THEN SRW_TAC [][]) THEN 
+  FIRST_X_ASSUM (Q.SPEC_THEN `SUC i` (MP_TAC o Q.GEN `i`)) THEN 
+  SIMP_TAC (srw_ss()) [] THEN 
+  `x + tyinst_sz h' + 1 + tylinst_sz xl = 
+     y + tyinst_sz h + 1 + tylinst_sz t` by DECIDE_TAC THEN 
+  `x + tyinst_sz h' + 1 <= y + tyinst_sz h + 1` by DECIDE_TAC THEN 
+  STRIP_TAC THEN 
+  `(x + tyinst_sz h' + 1 = y + tyinst_sz h + 1) /\ 
+   (tylinst_sz xl = tylinst_sz t)`
+     by METIS_TAC [] THEN 
+  DECIDE_TAC);
+  
 val type_match_size_eq_renaming = store_thm(
   "type_match_size_eq_renaming",
-  ``(!id1 s ty2. (cppid_inst s id1 = SOME ty2) /\
-                 (tyinst_sz ty2 = 1 + cppidinst_sz id1) ==>
-                 renaming_upto (cppidfrees id1) s) /\
-    (!sfld1 s sfld2. (sfld_inst s sfld1 = SOME sfld2) /\
-                     (sfldinst_sz sfld2 = sfldinst_sz sfld1) ==>
-                     renaming_upto (sfldfrees sfld1) s) /\
-    (!ta1 s ta2. (temparg_inst s ta1 = SOME ta2) /\
-                 (tainst_sz ta2 = tainst_sz ta1) ==>
-                 renaming_upto (tafrees ta1) s) /\
-    (!tva1 s tva2. (temp_valarg_inst s tva1 = SOME tva2) /\
-                   (tvainst_sz tva2 = tvainst_sz tva1) ==>
-                   renaming_upto (tvalfrees tva1) s) /\
-    (!ty1 s ty2. (type_inst s ty1 = SOME ty2) /\
+  ``(!s ty1 ty2. (type_inst s ty1 = SOME ty2) /\
                  (tyinst_sz ty2 = tyinst_sz ty1) ==>
                  renaming_upto (tyfrees ty1) s) /\
+    (!s id1 ty2. (cppid_inst s id1 = SOME ty2) /\
+                 (tyinst_sz ty2 = 1 + cppidinst_sz id1) ==>
+                 renaming_upto (cppidfrees id1) s) /\
+    (!s ta1 ta2. (temparg_inst s ta1 = SOME ta2) /\
+                 (tainst_sz ta2 = tainst_sz ta1) ==>
+                 renaming_upto (tafrees ta1) s) /\
+    (!s tva1 tva2. (temp_valarg_inst s tva1 = SOME tva2) /\
+                   (tvainst_sz tva2 = tvainst_sz tva1) ==>
+                   renaming_upto (tvalfrees tva1) s) /\
+    (!s sfld1 sfld2. (sfld_inst s sfld1 = SOME sfld2) /\
+                     (sfldinst_sz sfld2 = sfldinst_sz sfld1) ==>
+                     renaming_upto (sfldfrees sfld1) s) ``,
+  HO_MATCH_MP_TAC type_inst_ind THEN SRW_TAC [][] THEN 
+  FULL_SIMP_TAC (srw_ss()) [] THENL [
+    `cppidinst_sz id1 < tyinst_sz ty /\ tyinst_sz ty1 <= tyinst_sz y0` 
+       by METIS_TAC [type_match_size_increase] THEN 
+    IMP_RES_TAC typeid_size THEN 
+    SRW_TAC [ARITH_ss][],
+
+    `cppidinst_sz id1 < tyinst_sz ty /\ tyinst_sz ty1 <= tyinst_sz y0` 
+       by METIS_TAC [type_match_size_increase] THEN 
+    IMP_RES_TAC typeid_size THEN 
+    SRW_TAC [ARITH_ss][],
+
+    FULL_SIMP_TAC (srw_ss() ++ DNF_ss) [AND_IMP_INTRO, olmap_ALL_MEM] THEN
+    `(!i. i < LENGTH tylist ==> 
+          (tyinst_sz (EL i tylist) <= tyinst_sz (EL i y0))) /\
+     tyinst_sz ty1 <= tyinst_sz x0`
+       by METIS_TAC [type_match_size_increase] THEN 
+    
+    
+      
+    MATCH_MP_TAC renaming_upto_FOLDL THEN SRW_TAC [][] THENL [
+
+    SRW_TAC [][renaming_upto_def, tyfree_sing_def],
+
+    
+
+    
+      
+    `tyinst_sz ty = 1 + cppidinst_sz id` by 
+
+
     (!tal1 s tal2. (olmap (temparg_inst s) tal1 = SOME tal2) /\
                    (talinst_sz tal2 = talinst_sz tal1) ==>
                    renaming_upto (talfrees tal1) s) /\
